Paper stuff.

FraudProof/Games/Base/FMBC.lean
@@ -1,34 +1,35 @@
 import FraudProof.Games.Base.GenericTree -- Complex Strategies
 
-def cond_hash_elem {ℍ α : Type}[BEq ℍ][LawfulBEq ℍ][h : Hash α ℍ]
-  (leaf: ℍ) (rev : α) (res : ℍ)
-   : Bool :=  h.mhash rev == leaf && leaf == res
+def cond_hash_elem {α ℍ : Type}[BEq ℍ][LawfulBEq ℍ][h : Hash α ℍ]
+  (_leaf: Unit) (rev : α) (res : ℍ)
+   : Bool :=  h.mhash rev == res
 
 def cond_hash { ℍ : Type }[BEq ℍ][mag : HashMagma ℍ] (res l r : ℍ) : Bool
   := mag.comb l r == res
 
 -- Hash Game
 abbrev dac_game {ℍ α : Type}[BEq ℍ][LawfulBEq ℍ][Hash α ℍ][HashMagma ℍ]
-  (da : CompTree ℍ Unit ℍ)
-  (reveler : ABTree (Option α) (Option (ℍ × ℍ)))
+  (da : CompTree Unit Unit ℍ)
+  (revealer : ABTree (Option α) (Option (ℍ × ℍ)))
   (chooser : ABTree Unit ((ℍ × ℍ × ℍ) -> Option ChooserMoves))
   :=
-  treeCompArbGame cond_hash_elem (fun _ => cond_hash) da reveler chooser
+  treeCompArbGame cond_hash_elem (fun _ => cond_hash) da revealer chooser
 
 theorem winning_prop_hashes {ℍ α : Type}
-    [BEq ℍ][LawfulBEq ℍ]
+    [DecidableEq ℍ]
     [Hash α ℍ][HashMagma ℍ]
     -- Public Information
-    (da : CompTree ℍ Unit ℍ)
+    (da : CompTree Unit Unit ℍ)
     -- Players
-    (reveler : ABTree (Option α) (Option (ℍ × ℍ)))
-    (good_reveler : reveler_winning_condition cond_hash_elem (fun _ => cond_hash) da reveler)
+    (revealer : ABTree (Option α) (Option (ℍ × ℍ)))
+    (good_revealer : reveler_winning_condition cond_hash_elem (fun _ => cond_hash)
+                    da revealer)
     : forall (chooser : ABTree Unit ((ℍ × ℍ × ℍ) -> Option ChooserMoves)),
       treeCompArbGame
          cond_hash_elem (fun _ => cond_hash)
-         da reveler chooser
+         da revealer chooser
          = Player.Proposer
-    := winning_proposer_wins _ _ da reveler good_reveler
+    := winning_proposer_wins _ _ da revealer good_revealer
 
 def gen_chooser_opt {ℍ : Type}
    [DecidableEq ℍ]
@@ -43,29 +44,40 @@ def gen_chooser_opt {ℍ : Type}
           else .Continue .Right
    )
 
+def same_leaves {α β : Type}(revealer chooser : ABTree α β) : Prop
+ := match revealer, chooser with
+   | .leaf v , .leaf w => v = w
+   | .node _rn rl rr , .node _ln ll lr =>
+     same_leaves rl ll ∧ same_leaves rr lr
+   -- Isomorph
+   | _ , _ => False
+
+
 theorem winning_gen_chooser {ℍ α : Type}
-    [DecidableEq ℍ] -- Dec here hides collision free.
-    [h : Hash α ℍ][HashMagma ℍ]
+    [DecidableEq ℍ] [h : Hash α ℍ][HashMagma ℍ]
     -- Public Information
-    (pub_data : ABTree ℍ Unit)
+    (pub_data : ABTree Unit Unit)
     -- Players
-    (reveler : ABTree (Option α) (Option (ℍ × ℍ)))
-    (rev_res : ℍ)
-    --
-    (chooser : ABTree (Option α) (Option (ℍ × ℍ)))
-    (ch_res : ℍ)
-    (good_chooser: reveler_winning_condition cond_hash_elem (fun _ => cond_hash) ⟨ pub_data , ch_res ⟩ chooser)
+    (revealer : ABTree (Option α) (Option (ℍ × ℍ)))(rev_res : ℍ)
+    (chooser : ABTree (Option α) (Option (ℍ × ℍ)))(ch_res : ℍ)
+    -- Chooser knows the data and hashes do not match
+    (same_data : same_leaves revealer chooser)
+    (good_chooser: winning_condition_player
+                   (fun _ a h => @cond_hash_elem α ℍ _ _ _ () a h )
+                                      (fun _ (l,r) res => cond_hash res l r)
+                                      (fun _ x => x)
+                                      ⟨ pub_data , ch_res ⟩ chooser)
     (hneq : ¬ rev_res = ch_res)
     : treeCompArbGame
          cond_hash_elem (fun _ => cond_hash)
-         ⟨ pub_data, rev_res ⟩ reveler (chooser.map (fun _ => ()) gen_chooser_opt)
+         ⟨ pub_data, rev_res ⟩ revealer (chooser.map (fun _ => ()) gen_chooser_opt)
          = Player.Chooser
     := by
-  revert hneq good_chooser ch_res chooser rev_res reveler
+  revert hneq good_chooser same_data ch_res chooser rev_res revealer
   induction pub_data with
   | leaf v =>
-    intros reveler rev_res chooser ch_res good_ch hneq
-    cases reveler with
+    intros revealer rev_res chooser ch_res same_data good_ch hneq
+    cases revealer with
     | node _ _ _ => simp [treeCompArbGame]
     | leaf mrev =>
       cases mrev with
@@ -73,22 +85,21 @@ theorem winning_gen_chooser {ℍ α : Type}
       | some rev =>
         simp [treeCompArbGame]
         cases chooser with
-        | node _ _ _ => simp [reveler_winning_condition] at good_ch
+        | node _ _ _ => simp [winning_condition_player] at good_ch
         | leaf ch =>
         cases ch with
-        | none => simp [reveler_winning_condition] at good_ch
+        | none => simp [winning_condition_player] at good_ch
         | some ched =>
-          simp [reveler_winning_condition] at good_ch
+          simp [winning_condition_player] at good_ch
           unfold cond_hash_elem at *
           simp at good_ch
+          simp [same_leaves] at same_data
           simp
-          intro h
-          have ⟨ hchev , hvres ⟩ := good_ch
-          rw [hvres]
-          intro a; apply hneq; rw [a]
+          subst_eqs
+          intro pp; apply hneq; symm; assumption
   | node _ gl gr HIndL HIndR =>
-    intros reveler rev_res chooser ch_res good_ch hneq
-    cases reveler with
+    intros revealer rev_res chooser ch_res hsame good_ch hneq
+    cases revealer with
     | leaf _ => simp [treeCompArbGame]
     | node mp revl revr =>
       cases mp with
@@ -96,12 +107,12 @@ theorem winning_gen_chooser {ℍ α : Type}
       | some prop =>
         simp [treeCompArbGame]
         cases chooser with
-        | leaf _ => simp [reveler_winning_condition] at good_ch
+        | leaf _ => simp [winning_condition_player] at good_ch
         | node mch chl chr =>
           cases mch with
-          | none => simp [reveler_winning_condition] at good_ch
+          | none => simp [winning_condition_player] at good_ch
           | some ch =>
-            simp [reveler_winning_condition] at good_ch
+            simp [winning_condition_player] at good_ch
             simp [gen_chooser_opt]
             split
             case h_1 x heq =>
@@ -122,13 +133,17 @@ theorem winning_gen_chooser {ℍ α : Type}
                 rw [ite_eq_iff] at h_nonsense
                 simp at h_nonsense
             case h_2 x heq =>
-              apply HIndL; exact good_ch.2.1
+              apply HIndL
+              unfold same_leaves at hsame; exact hsame.1
+              exact good_ch.2.1
               simp at heq
               rw [ite_eq_iff] at heq
               simp at heq
               intro a; apply heq.2; rw [a]
             case h_3 x heq =>
-              apply HIndR; exact good_ch.2.2
+              apply HIndR
+              unfold same_leaves at hsame; exact hsame.2
+              exact good_ch.2.2
               simp at heq
               rw [ite_eq_iff] at heq
               simp at heq
